\documentclass[a4paper,11pt]{article}
\usepackage[utf8]{inputenc}
\usepackage{amsmath}
\usepackage{amsfonts}
\usepackage{amssymb}
\usepackage{graphicx}
\usepackage{braket}

\numberwithin{equation}{section}
\renewcommand\thesubsection{\alph{subsection}}
\newcommand{\bvp}[1]{\mathbf{#1}'}
\newcommand{\bv}[1]{\mathbf{#1}}


%opening
\title{Quantum III HW3}
\author{Vince Baker}

\begin{document}

\maketitle

\section{Problem 1}
We start with the double commutation relation $[[H,e^{ik\cdot r}],e^{ik\cdot r}]$. 
Following the usual proof of the Thomas-Reiche-Kuhn sum rule, we first write this as:
\begin{align}
 [H,e^{ik\cdot r}] &=  [\frac{p^2}{2m}+V(r),e^{ik\cdot r}]\\
 [H,e^{ik\cdot r}] &= \frac{-\hbar^2}{2m}\nabla^2(e^{ik\cdot r})+e^{ik\cdot r}\frac{\hbar^2}{2m}\nabla^2\\
 [[H,e^{ik\cdot r}],e^{ik\cdot r}] &= \frac{i\hbar k^2}{m}[p, r] = \frac{\hbar^2k^2}{m}
\end{align}
Now we expand the double commutator and write the expression for the final state:
\begin{align}
 &\bra{n}[He^{ik\cdot r}-e^{ik\cdot r}H,e^{ik\cdot r}]\ket{n}\\
 &2E_n\bra{n}e^{i2k\cdot r}\ket{n}-2\bra{n}e^{ik\cdot r}He^{ik\cdot r} \ket{n}\\
 \begin{split}
 &\sum_m 2E_n\bra{n}e^{ik\cdot r}\ket{m}\bra{m}e^{ik\cdot r}\ket{n}\\&\ -2\sum_m\bra{n}e^{ik\cdot r}\ket{m}\bra{m}H\ket{m}\bra{m}e^{ik\cdot r}\ket{n}
 \end{split}\\
 &\sum_m 2(E_n-E_m)\bra{n}e^{ik\cdot r}\ket{m}^2
\end{align}
Combining 3 and 7, interchanging m for n, we have shown:
\begin{align}
 \sum_n (E_n-E_m)\bra{n}e^{ik\cdot r}\ket{m}^2 &= \frac{\hbar^2k^2}{2m}
\end{align}

\section{Problem 2}
We first evaluate the commutator $[L_z,P_+]$, with $L_z=-i\hbar x\frac{\partial}{\partial y}+i\hbar y\frac{\partial}{\partial x}$
and $P_+=-i\hbar \frac{\partial}{\partial x}+\hbar \frac{\partial}{\partial y}$.
Opening up the commutator and operating on a test function f:
\begin{align}
 \begin{split}
 [L_z,P_+] = &-\hbar^2x\frac{\partial f}{\partial x \partial y}-i\hbar^2x\frac{\partial^2f}{\partial y^2}+\hbar^2y\frac{\partial^2f}{\partial x^2}+i\hbar^2y\frac{\partial^2f}{\partial x \partial y}\\
  &+\hbar^2\left(\frac{\partial f}{\partial y}+x\frac{\partial^2f}{\partial x \partial y} \right)-\hbar^2y\frac{\partial^2 f}{\partial x^2}+i\hbar^2x\frac{\partial^2 f}{\partial y^2}\\
  &-i\hbar^2\left(\frac{\partial f}{\partial x}+y\frac{\partial^2 f}{\partial x \partial y} \right)
 \end{split}\\
 [L_z,P_+] &= \hbar^2\frac{\partial}{\partial y}-i\hbar^2\frac{\partial}{\partial x} = \hbar P_x
\end{align}

\section{Problem 3}
We use the Born approximation with a spherically symmetric potential:
\begin{align}
 f(\theta) &= \frac{-2m}{\hbar^2 k}\int_0^\infty rV(r)\sin{(kr)} dr\\
 f(\theta) &= \frac{2mV_0}{\hbar^2 k}\int_0^\infty r \sin{(kr)} e^{-r/a}dr\\
 f(\theta) &= \frac{4mV_0}{\hbar^2}\frac{a^3}{\left(k^2a^2+1 \right)^2}\\
 \frac{d\sigma}{d\Omega} &= |f(\theta)|^2 = \left\{\frac{4mV_0}{\hbar^2}\frac{a^3}{\left(k^2a^2+1 \right)^2} \right\}^2
\end{align}
Where we have done the integral through table lookup.

\section{Problem 4}


\section{Problem 5}
To prove the optical theorem we will compare the form of the stationary wavefunction in both the plane wave and spherical wave bases,
making use of the expansion of the incoming wave $e^{ikz}$ in the spherical wave basis.
\begin{align}
 \Psi_{k}(r) &= e^{ikz}+\frac{e^{ikr}}{r}\ \text{ (Plane wave basis)}\\
 e^{ikz} &= \sum_{\ell=0}^\infty i^\ell\sqrt{4\pi(2\ell +1)}j_\ell(kr)Y_\ell^0(\theta)\ \text{(spherical basis)}
\end{align}
For a spherically symmetric potential the effect of scattering in the spherical basis is a phase shift in the radial part of the wavefunction.
The asymptotic form is (multiplying through by the phase shift):
\begin{align}
 U^{diff}(r) &= \sum_{\ell=0}^\infty i^\ell \sqrt{4\pi(2\ell +1)}Y_\ell^0(\theta) \frac{e^{-i(kr+\ell(\pi/2))}-e^{i(kr-\ell(\pi/2)+2\delta_\ell)}}{2ikr}
\end{align}
We can now add and subtract (2) from (3), and will get a form that we can compare to 1.
\begin{align}
 \begin{split}
 U^{diff}(r) = &e^{ikz} +\sum_{\ell=0}^\infty i^\ell \sqrt{4\pi(2\ell +1)}Y_\ell^0(\theta)\\
	       &X\left\{-\frac{e^{ikr}e^{i\ell(\pi/2)}}{2ikr}+\frac{e^{ikr}e^{i\ell(\pi/2)}e^{i2\delta_\ell}}{2ikr} \right\}
 \end{split}\\
 U^{diff}(r) = &e^{ikz} +\sum_{\ell=0}^\infty i^\ell \sqrt{4\pi(2\ell +1)}Y_\ell^0(\theta)\frac{e^{ikr}}{kr}e^{-i\ell(\pi/2)}\left(\frac{1-e^{i2\delta_\ell}}{2i} \right)\\
 U^{diff}(r) &= e^{ikz}+\sum_{\ell=0}^\infty i^\ell\sqrt{4\pi(2\ell+1)}\frac{e^{ikr}}{kr}e^{-i\ell(\pi/2)}e^{i\delta_\ell}\ \sin{\delta_\ell}Y_\ell^0(\theta)\\
 f(\theta,\phi) &= \frac{1}{k}\sum_\ell^\infty \sqrt{4\pi(2\ell+1)}Y_\ell^0(\theta)e^{i\delta_\ell}\sin{\delta_\ell}
\end{align}
Where we have used the fact that $e^{-i\ell(\pi/2)}=(-i)^\ell$ for $\ell=0,1,2...$ in the final step.
We can now compute $\sigma_{\text{total}}$ by taking the integral over all angles.
\begin{align}
 \sigma_{\text{total}} &= \int \mid f(\theta)\mid^2 d\Omega\\
 \begin{split}
 \sigma_{\text{total}} = &\int d\Omega Y_\ell^0 Y_{\ell^\prime}^0 \sum_\ell^\infty \sum_{\ell^\prime}^\infty \sqrt{4\pi(2\ell+1)}\sqrt{4\pi(2\ell^\prime+1)}\\
			  &\times \sin{\delta_\ell}\sin{\delta_{\ell^\prime}}
 \end{split}\\
 \sigma_{\text{total}} &= \frac{4\pi}{k^2}\sum_{\ell=0}^\infty (2\ell+1)\sin^2{\delta_\ell}
\end{align}
Where we have used the orthonormalization of the spherical harmonics $Y_\ell^0Y_{\ell^\prime}^0=\delta_{\ell\ell^\prime} $.\\
To prove the optical theorem, we compute the imaginary part of $f(\theta,\phi)$ at $\theta=0$.
Noting that $Y_\ell^0(1)=1$ for all $\ell$:
\begin{align}
 Im\left(f(\theta,\phi)\right) &= \frac{1}{k}\sum_{\ell=0}^\infty (2\ell+1)\sin{\delta_\ell}\ Im\left(e^{i\delta_\ell}\right)\\
 Im\left(f(\theta,\phi)\right) &= \frac{1}{k}\sum_{\ell=0}^\infty (2\ell+1)\sin^2{\delta_\ell}
\end{align}
Comparing with (10) we have proved the optical theorem:
\begin{align}
 \sigma_{\text{total}} &= \frac{4\pi}{k}\ Im\left(f(\theta,\phi)|_{\theta=0} \right)
\end{align}


\end{document}
